StAM.v
@@ -4,7 +4,7 @@ Definition BS := nat.
 
 (* Specific AM monad state *)
 Record AM_St : Type := mkAM_St
-                         { am_nonceMap : Map nat BS;
+                         { am_nonceMap : Map (*Map nat BS*);
                            am_nonceId : nat;
                            checked : list nat }.
                                          
