StVM.v
@@ -3,7 +3,7 @@ Require Import Maps.
 
 (* Specific VM monad state *)
 Definition ev_stack := gen_stack EvidenceC.
-Definition ev_store := Map nat EvidenceC.
+Definition ev_store := Map.
 Record vm_st : Type := mk_st
                          {st_ev:EvidenceC ;
                           st_stack:ev_stack ; 
